wip proofs for wp

deps/poulet4/lib/P4automata/Bisimulations/AlgorithmicLeapsProofs.v
@@ -21,12 +21,105 @@ Section AlgorithmicLeaps.
                           S q1 q2)
                         (at level 40).
 
+  Definition bisimulation_with_leaps (R: rel conf) :=
+    forall q1 q2 : configuration a,
+      R q1 q2 ->
+      (accepting q1 <-> accepting q2) /\
+      (forall buf : list bool,
+          length buf = Nat.min (configuration_room_left q1) (configuration_room_left q2) ->
+          R (follow q1 buf) (follow q2 buf)).
+
+  Lemma bisimilar_is_bisimulation:
+    forall R q1 q2,
+      bisimulation_with_leaps R ->
+      R q1 q2 ->
+      Leaps.bisimilar_with_leaps a q1 q2.
+  Proof.
+    cofix C.
+    intros.
+    constructor.
+    - specialize (H q1 q2 H0).
+      tauto.
+    - intros.
+      eapply C with (R:=R); auto.
+      apply H; eauto.
+  Qed.
+
+  Definition follow_closed (R T: rel conf) : Prop :=
+    forall q1 q2,
+      R q1 q2 ->
+      forall bs,
+        length bs = Nat.min (configuration_room_left q1)
+                            (configuration_room_left q2) ->
+        (relation_conjunction R T) (follow q1 bs) (follow q2 bs).
+
+  Definition coaccepting (R: rel conf) : Prop :=
+    forall q1 q2,
+      R q1 q2 ->
+      (accepting q1 <-> accepting q2).
+
+  Lemma pre_bisimulation_is_bisimulation:
+    forall R T,
+      coaccepting (⟦R⟧ ⊓ ⟦T⟧) ->
+      follow_closed ⟦R⟧ ⟦T⟧ ->
+      bisimulation_with_leaps (pre_bisimulation a top R T).
+  Proof.
+    unfold bisimulation_with_leaps.
+    intros.
+    induction H1.
+    - split.
+      + apply H; split; auto.
+        simpl.
+        eapply interp_rels_bound; eauto.
+      + intros.
+        constructor.
+        unfold follow_closed in H0.
+        apply H; auto.
+    - split.
+      + apply H; split; auto.
+        simpl.
+        eapply interp_rels_bound; eauto.
+      + admit.
+      + intros.
+        unfold follow_closed in H.
+        constructor 2.
+        auto.
+        apply IHpre_bisimulation; auto.
+        unfold follow_closed; intros.
+        split; eapply H; eauto.
+    - split.
+      + admit.
+      + intros.
+        unfold follow_closed in H.
+        econstructor 3.
+        * eauto.
+        * eapply IHpre_bisimulation; auto.
+          unfold follow_closed; intros.
+          destruct H4.
+          repeat split; eauto.
+          -- eapply H; eauto.
+          -- eapply H; eauto.
+          -- eapply interp_rels_app; try solve [eapply H; eauto].
+             admit.
+        * intros.
+          eapply H2; eauto.
+  Admitted.
+  
   Lemma algorithmic_leaps_implies_bisimilar_leaps:
     forall R T q1 q2,
       pre_bisimulation a top R T q1 q2 ->
       Leaps.bisimilar_with_leaps a q1 q2.
   Proof.
     intros.
+    eapply bisimilar_is_bisimulation.
+    cofix C.
+    constructor.
+    induction H.
+    - 
+    - cofix C.
+    constructor.
+    - inversion H0.
+    - 
   Abort.
   
 End AlgorithmicLeaps.
